src/Config.fsti
@@ -32,8 +32,19 @@ val alg_null: v:nat{v = US.v metadata_max + 1}
 noextract inline_for_extraction
 val alg_null_sizet: v:US.t{US.v v = US.v metadata_max + 1}
 
-//TODO: use  this variable
+// guard pages mechanism
+// given the slab allocator memory layout,
+// is required to avoid basic large buffer overflows
+// actually, this flag controls whether guard pages are unmapped
 inline_for_extraction
 val enable_guard_pages: bool
 inline_for_extraction
 val guard_pages_interval: v:US.t{2 <= US.v v /\ US.fits (US.v metadata_max + US.v v)}
+
+// quarantine mechanism
+// for now, basic quarantine:
+// when a slab becomes empty (from partial/full),
+// it is never used again
+// actually, this flag controls whether quarantined slabs are unmapped
+inline_for_extraction
+val enable_quarantine: bool
