src/MemoryTrap.fsti
@@ -1,4 +1,4 @@
-module Guards
+module MemoryTrap
 
 open Utils2
 open SlotsAlloc
@@ -15,44 +15,24 @@ module A = Steel.Array
 module G = FStar.Ghost
 
 open Config
-open MemoryTrap
 
-val is_guard
+val is_trap
   (size_class: sc)
   (arr: array U8.t{A.length arr = U32.v page_size})
   (md: slab_metadata)
   (x: normal (t_of (slab_vprop size_class arr md)))
   : prop
 
-let trap_implies_guard
-  (size_class: sc)
-  (arr: array U8.t{A.length arr = U32.v page_size})
-  (md: slab_metadata)
-  (x: normal (t_of (slab_vprop size_class arr md)))
-  : Lemma
-  (requires is_trap size_class arr md x)
-  (ensures is_guard size_class arr md x)
-  = admit ()
-
-let mmap_trap_guard
+//assumed implementation is written in C
+val mmap_trap
   (size_class: G.erased sc)
   (arr: array U8.t{A.length arr = U32.v page_size})
   (md: G.erased (array U64.t){A.length md = 4})
-  (len: US.t{US.v len = U32.v page_size})
   : Steel unit
   (slab_vprop size_class arr md)
   (fun _ -> slab_vprop size_class arr md)
   (requires fun _ -> True)
   (ensures fun _ _ h1 ->
     let v = h1 (slab_vprop size_class arr md) in
-    is_guard size_class arr md v
-  )
-  =
-  if enable_guard_pages then (
-    mmap_trap size_class arr md;
-    let v = gget (slab_vprop size_class arr md) in
-    trap_implies_guard size_class arr md v
-  ) else (
-    let v = gget (slab_vprop size_class arr md) in
-    assume (is_guard size_class arr md v)
+    is_trap size_class arr md v
   )
